compiler/backend/proofs/source_to_flatProofScript.sml
@@ -3752,32 +3752,10 @@ val compile_correct = Q.store_thm("compile_correct",
 open flat_uncheck_ctorsProofTheory flat_elimProofTheory
      flat_exh_matchProofTheory flat_reorder_matchProofTheory
 
-(* TODO move to flat_exh_matchProofTheory *)
-val get_tdecs_thm = Q.store_thm("get_tdecs_thm",
-  `!xs.
-     get_tdecs xs =
-       MAP (\d. case d of Dtype t s => t)
-           (FILTER (\d. ?t s. d = Dtype t s) xs)`,
-  Induct \\ rw [get_tdecs_def] \\ fs []
-  \\ Cases_on `h` \\ fs []);
-
-(* TODO move to flat_exh_matchProofTheory *)
-val get_tdecs_APPEND = Q.store_thm("get_tdecs_APPEND",
-  `get_tdecs (xs ++ ys) = get_tdecs xs ++ get_tdecs ys`,
-  Induct_on `xs` \\ rw [get_tdecs_def]
-  \\ every_case_tac \\ fs []);
-
-(* TODO move to flat_exh_matchProofTheory *)
-val get_tdecs_MEM = Q.store_thm("get_tdecs_MEM",
-  `!xs. MEM t (get_tdecs xs) <=> ?s. MEM (Dtype t s) xs`,
-  Induct \\ rw [get_tdecs_def]
-  \\ Cases_on `h` \\ fs []
-  \\ metis_tac []);
-
 (* TODO move *)
-val FILTER3_T = Q.store_thm ("FILTER3_T",
-  `FILTER (\(x,y,z). T) xs = xs`,
-  Induct_on `xs` \\ rw [] \\ fs [ELIM_UNCURRY]);
+val FILTER_T = Q.store_thm ("FILTER_T",
+  `FILTER (\x. T) xs = xs`,
+  Induct_on `xs` \\ rw [] \\ fs []);
 
 (* source_to_flat$compile_decs always generates fresh type identifiers,
    so they must be unique. *)
@@ -3791,54 +3769,30 @@ val compile_decs_tidx_thm = Q.store_thm("compile_decs_tidx_thm",
   ho_match_mp_tac compile_decs_ind
   \\ rw [compile_decs_def] \\ fs [get_tdecs_def]
   \\ rpt (pairarg_tac \\ fs []) \\ rw []
-  \\ fs [get_tdecs_APPEND, ALL_DISTINCT_APPEND]
-  \\ TRY (EVAL_TAC \\ NO_TAC)
-  \\ TRY (fs [get_tdecs_thm, MAPi_enumerate_MAP, FILTER_MAP, MAP_MAP_o,
-              o_DEF, UNCURRY] \\ NO_TAC)
-  \\ TRY (fs [EVERY_MEM, MEM_MAPi, UNCURRY] \\ rw [] \\ NO_TAC)
-  \\ TRY
-   (fs [EVERY_MEM] \\ rw [] \\ fs []
-    \\ res_tac \\ fs []
-    \\ imp_res_tac compile_decs_num_bindings \\ fs []
-    \\ NO_TAC)
+  \\ fs [FILTER_APPEND, ALL_DISTINCT_APPEND, compile_exp_def,
+         MAPi_enumerate_MAP, FILTER_MAP, MAP_MAP_o, o_DEF, UNCURRY,
+         EVERY_MEM, MEM_MAPi] \\ rw []
+  \\ fs [FILTER_T, MAP_enumerate_MAPi, LAMBDA_PROD]
   >-
-   (fs [get_tdecs_thm, MAPi_enumerate_MAP, MAP_MAP_o, FILTER_MAP, o_DEF,
-        LAMBDA_PROD, FILTER3_T]
-    \\ fs [MAP_enumerate_MAPi]
-    \\ rename1 `_ + x`
-    \\ map_every qid_spec_tac [`x`, `type_def`]
-    \\ Induct \\ rw []
-    \\ fs [o_DEF, ADD1]
-    >- (strip_tac \\ fs [MEM_MAPi, ELIM_UNCURRY])
+   (rename1 `_ + x`
+    \\ map_every qid_spec_tac [`x`,`type_def`]
+    \\ Induct \\ rw [MEM_MAPi]
+    \\ fs [ELIM_UNCURRY, o_DEF, ADD1]
     \\ first_x_assum (qspec_then `x + 1` assume_tac)
     \\ once_rewrite_tac [DECIDE ``x + (n + 1) = n + (x + 1n)``] \\ fs [])
   >-
-   (rw [EVERY_MEM, MEM_MAPi, ELIM_UNCURRY]
-    \\ fs [])
+   (rename1 `_ + x`
+    \\ map_every qid_spec_tac [`x`,`type_def`]
+    \\ Induct \\ rw [miscTheory.enumerate_def])
+  \\ fs [GSYM get_tdecs_def]
+  \\ imp_res_tac get_tdecs_MEM \\ fs []
+  \\ res_tac \\ fs []
+  \\ imp_res_tac compile_decs_num_bindings \\ fs []
   >-
-   (Cases_on `type_def`
-    \\ fs [get_tdecs_def, ELIM_UNCURRY])
-  >-
-   (rw [] \\ strip_tac
-    \\ fs [EVERY_MEM]
+   (strip_tac
     \\ imp_res_tac get_tdecs_MEM \\ fs []
     \\ res_tac \\ fs [])
-  \\ eq_tac \\ rw [] \\ fs []
-  \\ simp [get_tdecs_thm, FILTER_EQ_NIL, EVERY_MEM]
-  \\ rw []
-  \\ strip_tac \\ fs [] \\ rveq
-  \\ `next1.tidx <> next1'.tidx`
-    by (strip_tac \\ rfs [] \\ fs []
-        \\ imp_res_tac get_tdecs_MEM
-        \\ rfs [])
-  \\ imp_res_tac compile_decs_num_bindings \\ fs []);
-
-val compile_tidx_thm = Q.store_thm("compile_tidx_thm",
-  `compile c1 ds1 = (c2, ds2) ==> ALL_DISTINCT (get_tdecs ds2)`,
-  rw [compile_def]
-  \\ pairarg_tac \\ fs []
-  \\ imp_res_tac compile_decs_tidx_thm \\ fs [] \\ rveq
-  \\ fs [glob_alloc_def, get_tdecs_def]);
+  \\ eq_tac \\ rw [] \\ fs []);
 
 val compile_flat_correct = Q.store_thm("compile_flat_correct",
   `precondition s env c /\
@@ -3861,12 +3815,16 @@ val compile_prog_semantics = Q.store_thm("compile_prog_semantics",
    ¬semantics_prog s env prog Fail ⇒
    semantics_prog s env prog (semantics T F s.ffi (SND (compile_prog c prog)))`,
   rw [compile_prog_def] \\ pairarg_tac \\ fs []
-  \\ imp_res_tac compile_tidx_thm
   \\ imp_res_tac compile_correct \\ rfs []
   \\ `semantics F T s.ffi p' <> Fail` by (CCONTR_TAC \\ fs [])
   \\ `semantics F T s.ffi p' = semantics T F s.ffi (compile_flat p')`
     suffices_by (rw []\\ fs [])
   \\ match_mp_tac compile_flat_correct \\ fs []
+  \\ fs [compile_def]
+  \\ pairarg_tac \\ fs [] \\ rveq
+  \\ imp_res_tac compile_decs_tidx_thm
+  \\ fs [glob_alloc_def, get_tdecs_def]
+  \\ fs [GSYM glob_alloc_def, GSYM get_tdecs_def]
   \\ rw [EVERY_MEM, is_new_type_def]
   \\ strip_tac
   \\ `tid <> 0 ==> tid = 1`
@@ -3878,10 +3836,7 @@ val compile_prog_semantics = Q.store_thm("compile_prog_semantics",
         \\ qpat_x_assum `FDOM _ = _` mp_tac
         \\ EVAL_TAC \\ fs [flookup_thm] \\ rw []
         \\ CCONTR_TAC \\ fs [])
-  \\ fs [compile_def]
-  \\ pairarg_tac \\ fs [] \\ rveq
-  \\ imp_res_tac compile_decs_tidx_thm \\ fs [glob_alloc_def]
-  \\ fs [EVERY_MEM]
+  \\ fs [glob_alloc_def, EVERY_MEM]
   \\ res_tac \\ fs []);
 
 val _ = export_theory ();
